easy cases of StackMachComp.I_sim

src/StackMachComp.v
@@ -3,6 +3,7 @@ Require Import Metadata.
 Require String.
 Require ValueFlag StackMach.
 Require Import ListLemmas.
+Require Import HigherValue.
 
 Require Import Psatz.
 
@@ -42,4 +43,191 @@ Ltac refold_compile :=
     fold compile_list in *.
 
 
+Inductive I_expr (stk : list value) : A.expr -> list B.insn -> Prop :=
+| IArg : I_expr stk A.Arg [B.Arg]
+| ISelf : I_expr stk A.Self [B.Self]
 
+| IDeref1 : forall e code off,
+        I_expr [] e code ->
+        I_expr stk (A.Deref e off) [B.Block code; B.Deref off]
+| IDeref2 : forall v off,
+        nth_error stk 0 = Some v ->
+        I_expr stk (A.Deref (A.Value v) off) [B.Deref off]
+
+| ICall1 : forall f fcode a acode,
+        I_expr [] f fcode ->
+        I_expr [] a acode ->
+        I_expr stk (A.Call f a) [B.Block fcode; B.Block acode; B.Call]
+| ICall2 : forall fv a acode,
+        nth_error stk 0 = Some fv ->
+        I_expr [] a acode ->
+        I_expr stk (A.Call (A.Value fv) a) [B.Block acode; B.Call]
+| ICall3 : forall fv av,
+        nth_error stk 1 = Some fv ->
+        nth_error stk 0 = Some av ->
+        I_expr stk (A.Call (A.Value fv) (A.Value av)) [B.Call]
+
+| IMkConstr : forall tag vs es codes,
+        rev (firstn (length vs) stk) = vs ->
+        Forall2 (I_expr []) es codes ->
+        I_expr stk (A.MkConstr tag (map A.Value vs ++ es))
+                   (map B.Block codes ++ [B.MkConstr tag (length vs + length es)])
+
+| ISwitch : forall acases bcases,
+        Forall2 (I_expr []) acases bcases ->
+        I_expr stk (A.Switch acases) [B.Switch bcases]
+
+| IMkClose : forall fname vs es codes,
+        rev (firstn (length vs) stk) = vs ->
+        Forall2 (I_expr []) es codes ->
+        I_expr stk (A.MkClose fname (map A.Value vs ++ es))
+                   (map B.Block codes ++ [B.MkClose fname (length vs + length es)])
+.
+
+Inductive I : A.state -> B.state -> Prop :=
+| IRun : forall ae aa as_ ak  bcode bf bk,
+        I_expr (B.stack bf) ae bcode ->
+        aa = B.arg bf ->
+        as_ = B.self bf ->
+        (forall v, I (ak v) (bk v)) ->
+        I (A.Run ae aa as_ ak) (B.Run bcode bf bk)
+
+| IStop : forall v,
+        I (A.Stop v) (B.Stop v).
+
+
+
+Lemma stack_app_I_expr : forall stk stk' a b,
+    I_expr stk a b ->
+    I_expr (stk ++ stk') a b.
+inversion 1; constructor; eauto.
+- rewrite nth_error_app1 by (rewrite <- nth_error_Some; congruence). auto.
+- rewrite nth_error_app1 by (rewrite <- nth_error_Some; congruence). auto.
+- rewrite nth_error_app1 by (rewrite <- nth_error_Some; congruence). auto.
+- rewrite nth_error_app1 by (rewrite <- nth_error_Some; congruence). auto.
+
+- rewrite firstn_app; auto.
+  on (_ = vs), fun H => rewrite <- H.
+  rewrite rev_length. rewrite firstn_length. lia.
+- rewrite firstn_app; auto.
+  on (_ = vs), fun H => rewrite <- H.
+  rewrite rev_length. rewrite firstn_length. lia.
+Qed.
+Hint Resolve stack_app_I_expr.
+
+Lemma stack_nil_I_expr : forall stk a b,
+    I_expr [] a b ->
+    I_expr stk a b.
+intros. change stk with ([] ++ stk). eapply stack_app_I_expr. auto.
+Qed.
+Hint Resolve stack_nil_I_expr.
+
+
+
+Theorem compile_I_expr : forall a b,
+    A.no_values a ->
+    compile a = b ->
+    I_expr [] a b.
+induction a using A.expr_rect_mut with
+    (Pl := fun a => forall b,
+        A.no_values_list a ->
+        compile_list a = b ->
+        Forall2 (I_expr []) a b);
+intros0 Hnval Hcomp;
+simpl in Hcomp; refold_compile; try (rewrite <- Hcomp; clear Hcomp);
+simpl in Hnval; A.refold_no_values; repeat break_and;
+try solve [econstructor; eauto].
+
+- (* Value *) invc Hnval.
+- (* MkConstr *)
+  eapply IMkConstr with (vs := []); eauto.
+- (* MkClose *)
+  eapply IMkClose with (vs := []); eauto.
+Qed.
+
+
+Lemma I_expr_not_value : forall stk a b,
+    I_expr stk a b ->
+    ~ A.is_value a.
+inversion 1; inversion 1.
+Qed.
+Hint Resolve I_expr_not_value.
+
+Lemma I_expr_not_value' : forall stk a b,
+    I_expr stk a b ->
+    A.is_value a ->
+    False.
+intros. eapply I_expr_not_value; eauto.
+Qed.
+Hint Resolve I_expr_not_value'.
+
+Ltac i_ctor := intros; constructor; eauto.
+Ltac i_lem H := intros; eapply H; eauto.
+
+Theorem I_sim : forall AE BE a a' b,
+    Forall2 (I_expr []) AE BE ->
+    I a b ->
+    A.sstep AE a a' ->
+    exists b',
+        B.sstep BE b b' /\
+        I a' b'.
+
+destruct a as [ae al ak | ae];
+intros0 Henv II Astep; [ | solve [invc Astep] ].
+
+inv Astep; invc II; try on (I_expr _ _ _), invc.
+(* Kill off some bogus cases *)
+all: try solve [on (~ A.is_value _), contradict; constructor].
+all: try solve [on (I_expr _ (A.Value _) _), inv].
+all: try solve [exfalso; eauto].
+
+- (* Arg *)
+  eexists. split. eapply B.SArg.
+  on _, eapply_.
+
+- (* Self *)
+  eexists. split. eapply B.SSelf.
+  on _, eapply_.
+
+- (* DerefStep *)
+  eexists. split. eapply B.SBlock.
+  i_ctor. i_ctor. i_ctor.
+
+- (* DerefinateConstr *)
+  eexists. split. eapply B.SDerefinateConstr; eauto.
+  on _, eapply_.
+
+- (* DerefinateClose *)
+  eexists. split. eapply B.SDerefinateClose; eauto.
+  on _, eapply_.
+
+- (* ConstrStep *)
+  admit.
+
+- (* ConstrDone *)
+  admit.
+
+- (* CloseStep *)
+  admit.
+
+- (* CloseDone *)
+  admit.
+
+- (* CallL *)
+  eexists. split. eapply B.SBlock.
+  i_ctor. i_ctor. i_ctor.
+
+- (* CallR *)
+  eexists. split. eapply B.SBlock.
+  i_ctor. i_ctor. i_ctor.
+
+- (* MakeCall *)
+  fwd eapply Forall2_nth_error_ex as HH; eauto.  destruct HH as (bbody & ? & ?).
+  eexists. split. eapply B.SMakeCall; eauto.
+  i_ctor.
+
+- (* Switchinate *)
+  fwd eapply Forall2_nth_error_ex as HH; eauto.  destruct HH as (bcase & ? & ?).
+  eexists. split. eapply B.SSwitchinate; eauto.
+  i_ctor.
+Admitted.
